aneris/aneris_lang/state_interp/state_interp.v
@@ -73,134 +73,27 @@ Section state_interpretation.
     iApply (mapsto_node_valid_sockets with "[$] [$]").
   Qed.
 
+  (* TODO: define this - Becomes trivial with new approach to ports *)
   Definition addrs_to_ip_ports_map (A : gset socket_address) :
-    gmap ip_address (gset port) :=
-    ∅.
-
-  (** free_ips_coh *)
-  Lemma free_ips_coh_init ips Ps σ :
-    dom Ps ## ips →
-    (∀ ip, ip ∈ ips → ip_is_free ip σ) →
-    ((∀ ip ps, Ps !! ip = Some (GSet ps) →
-              ∀ Sn, (state_sockets σ) !! ip = Some Sn →
-                    ∀ p, p ∈ ps → port_not_in_use p Sn)) →   
-    free_ips_auth ips ∗ free_ports_auth Ps -∗
-    free_ips_coh σ.
-  Proof.
-    iIntros (Hdisj Hip Hnuse) "[HipsCtx HPiu]".
-    iExists _, _; iFrame.
-    iPureIntro. done.
-  Qed.
-
-  (* (* aneris_state_interp *) *)
-  (* Lemma aneris_state_interp_init A fips σ γs : *)
-  (*   (* Free Ips [fips] are disjoint from initial allocted nodes *)
-  (*      [dom (state_heaps σ]) *) *)
-  (*   fips ## dom (state_heaps σ) → *)
-  (*   (* dom (addrs_to_ip_ports_map (union_set A)) → *) *)
-  (*   (∀ ip : ip_address, ip ∈ fips → ip_is_free ip σ) → *)
-  (*   dom (state_sockets σ) = dom (state_heaps σ) → *)
-  (*   dom γs =dom (state_heaps σ) → *)
-  (*   dom (state_heaps σ) = dom (addrs_to_ip_ports_map (union_set A)) → *)
-  (*   dom (state_sockets σ) = dom (addrs_to_ip_ports_map (union_set A)) → *)
-  (*   map_Forall (λ _ σh, σh = ∅) (state_heaps σ) → *)
-  (*   map_Forall (λ _ skts, skts = ∅) (state_sockets σ) → *)
-  (*   state_ms σ = ∅ → *)
-  (*   node_gnames_auth γs -∗ *)
-  (*   ([∗ map] ip↦γ ∈ γs, mapsto_node ip γ ∗ heap_ctx γ ∅ ∗ sockets_ctx γ ∅) -∗ *)
-  (*   messages_ctx (gset_to_gmap (∅, ∅) A)  -∗ *)
-  (*   socket_address_group_ctx A -∗ *)
-  (*   unallocated_groups_auth A -∗ *)
-  (*   saved_si_auth ∅ -∗ *)
-  (*   free_ips_auth fips -∗ *)
-  (*   free_ports_auth (GSet <$> addrs_to_ip_ports_map (union_set A)) -∗ *)
-  (*   aneris_state_interp σ (∅, ∅). *)
-  (* Proof. *)
-  (*    iIntros (Hfips Hfips' Hfips'' Hheap Hskt Hheaps Hskts Hms) *)
-  (*           "Hγs_auth Hγs Hm Hsags Hunallocated Hsif HipsCtx HPiu_auth". *)
-  (*   iDestruct (socket_address_group_ctx_valid with "Hsags") as %[Hdisj Hne]. *)
-  (*   iExists _, _; iFrame. *)
-  (*   iSplit. *)
-  (*   (* messages_received_sent *) *)
-  (*   { iPureIntro. apply messages_received_sent_init. } *)
-  (*   iSplit. *)
-  (*   (* gnames_coh *) *)
-  (*   { iPureIntro. *)
-  (*     (* TODO: Dont break abstraction here. *) *)
-  (*     by rewrite /gnames_coh Hheap Hskt. } *)
-  (*   iSplitR. *)
-  (*   (* network_sockets_coh *) *)
-  (*   { iPureIntro. *)
-  (*     (* TODO: Dont break abstraction here. *) *)
-  (*     rewrite /network_sockets_coh. *)
-  (*     intros ip Sn HSome. apply Hskts in HSome as ->. *)
-  (*     split. *)
-  (*     { rewrite /socket_handlers_coh. set_solver. } *)
-  (*     split. *)
-  (*     { rewrite /socket_messages_coh. set_solver. } *)
-  (*     split. *)
-  (*     { rewrite /socket_addresses_coh. set_solver. } *)
-  (*     rewrite /socket_unbound_empty_buf_coh. set_solver. } *)
-  (*   iSplitR. *)
-  (*   (* messages_history_coh *) *)
-  (*   { iPureIntro. *)
-  (*     (* TODO: Dont break abstraction here. *) *)
-  (*     rewrite /messages_history_coh. rewrite Hms. *)
-  (*     split. *)
-  (*     { rewrite /message_soup_coh. set_solver. } *)
-  (*     split. *)
-  (*     { rewrite /receive_buffers_coh. *)
-  (*       intros ip Sn sh skt r m HSome. apply Hskts in HSome as ->. *)
-  (*       set_solver. } *)
-  (*     split. *)
-  (*     { rewrite /messages_addresses_coh. *)
-  (*       rewrite dom_gset_to_gmap. *)
-  (*       split; [done|]. *)
-  (*       split; [set_solver|]. *)
-  (*       intros sag R T HSome. rewrite lookup_gset_to_gmap_Some in HSome. *)
-  (*       destruct HSome. set_solver. } *)
-  (*     rewrite /messages_received_from_sent_coh. *)
-  (*     rewrite messages_received_init messages_sent_init. set_solver. } *)
-  (*   (* socket_interp_coh *) *)
-  (*   iDestruct (socket_address_groups_ctx_own with "Hsags") as "#Hsags'". *)
-  (*   iSplitL "Hsags Hunallocated Hsif". *)
-  (*   { by iApply (socket_interp_coh_init with "Hsags Hunallocated Hsif"). } *)
-  (*   iSplitL "Hγs". *)
-  (*   (* local_state_coh *) *)
-  (*   { iApply (big_sepM_impl with "Hγs"). *)
-  (*     iIntros "!>" (k x HSome) "(Hnode & Hheap & Hskt)". *)
-  (*     assert (is_Some ((state_heaps σ) !! k)) as [y HSomey]. *)
-  (*     { apply elem_of_dom. rewrite Hheap. apply elem_of_dom. by exists x. } *)
-  (*     assert (is_Some ((state_sockets σ) !! k)) as [z HSomez]. *)
-  (*     { apply elem_of_dom. rewrite Hskt. apply elem_of_dom. by exists x. } *)
-  (*     iExists _, _. *)
-  (*     iSplit; [done|].  *)
-  (*     iSplit; [done|]. *)
-  (*     apply Hheaps in HSomey as ->. *)
-  (*     apply Hskts in HSomez as ->. *)
-  (*     rewrite fmap_empty. *)
-  (*     iFrame. } *)
-  (*   iSplitL "HipsCtx HPiu_auth". *)
-  (*   (* free_ips_coh *) *)
-  (*   { by iApply (free_ips_coh_init with "[$]"). } *)
-  (*   (* messages_resource_coh *) *)
-  (*   iApply messages_resource_coh_init. *)
-  (*   iFrame "#". *)
-  (* Qed. *)
-
+    gmap ip_address (gset port) := ∅.
 
   (* aneris_state_interp *)
-  Lemma aneris_state_interp_init fips A σ γs :
+  Lemma aneris_state_interp_init_strong fips A σ γs :
     fips ## dom γs →
     fips ## dom (addrs_to_ip_ports_map (union_set A)) →
     (∀ ip : ip_address, ip ∈ fips → ip_is_free ip σ) →
     dom (state_heaps σ) = dom γs →
     dom (state_sockets σ) = dom γs →
-    map_Forall (λ _ σh, σh = ∅) (state_heaps σ) →
-    map_Forall (λ _ skts, skts = ∅) (state_sockets σ) →
+    (* map_Forall (λ _ σh, σh = ∅) (state_heaps σ) → *)
+    map_Forall (λ ip s, map_Forall (λ sh sb, sb.2 = []) s) (state_sockets σ) →
+    map_Forall (λ ip s, socket_handlers_coh s) (state_sockets σ) →
+    map_Forall (λ ip s, socket_addresses_coh s ip) (state_sockets σ) →
+    (* map_Forall (λ _ skts, skts = ∅) (state_sockets σ) → *)
     state_ms σ = ∅ →
     node_gnames_auth γs -∗
-    ([∗ map] ip↦γ ∈ γs, mapsto_node ip γ ∗ heap_ctx γ ∅ ∗ sockets_ctx γ ∅) -∗
+    ([∗ map] ip↦γ ∈ γs, mapsto_node ip γ ∗
+                        heap_ctx γ (state_heaps σ !!! ip) ∗
+                        sockets_ctx γ (fst <$> (state_sockets σ !!! ip))) -∗
     messages_ctx (gset_to_gmap (∅, ∅) A)  -∗
     socket_address_group_ctx A -∗
     unallocated_groups_auth A -∗
@@ -211,7 +104,7 @@ Section state_interpretation.
     (*    free_ports ip ports)%I -∗ *)
     aneris_state_interp σ (∅, ∅).
   Proof.
-     iIntros (Hfips Hfips' Hfips'' Hheap Hskt Hheaps Hskts Hms)
+     iIntros (Hfips Hfips' Hfips'' Hheap Hskt Hskts Hskts_coh1 Hskts_coh2 Hms)
             "Hγs_auth Hγs Hm Hsags Hunallocated Hsif HipsCtx HPiu_auth".
     iDestruct (socket_address_group_ctx_valid with "Hsags") as %[Hdisj Hne].
     iExists _, _; iFrame.
@@ -228,14 +121,20 @@ Section state_interpretation.
     { iPureIntro.
       (* TODO: Dont break abstraction here. *)
       rewrite /network_sockets_coh.
-      intros ip Sn HSome. apply Hskts in HSome as ->.
+      intros ip Sn HSome.
       split.
-      { rewrite /socket_handlers_coh. set_solver. }
+      { by apply Hskts_coh1 in HSome. } (* TODO: Dont take as input *)
       split.
-      { rewrite /socket_messages_coh. set_solver. }
+      { apply Hskts in HSome.
+        rewrite /socket_messages_coh.
+        intros sh skt r sa HSn. apply HSome in HSn. simpl in *.
+        simplify_eq. set_solver. }
       split.
-      { rewrite /socket_addresses_coh. set_solver. }
-      rewrite /socket_unbound_empty_buf_coh. set_solver. }
+      { by apply Hskts_coh2 in HSome. } (* TODO: Dont take as input *)
+      apply Hskts in HSome.
+      rewrite /socket_unbound_empty_buf_coh.
+      intros sh skt r HSn. apply HSome in HSn. simpl in *.
+      simplify_eq. done. }
     iSplitR.
     (* messages_history_coh *)
     { iPureIntro.
@@ -245,7 +144,8 @@ Section state_interpretation.
       { rewrite /message_soup_coh. set_solver. }
       split.
       { rewrite /receive_buffers_coh.
-        intros ip Sn sh skt r m HSome. apply Hskts in HSome as ->.
+        intros ip Sn sh skt r m HSome. apply Hskts in HSome.
+        intro HSn. apply HSome in HSn.
         set_solver. }
       split.
       { rewrite /messages_addresses_coh.
@@ -269,15 +169,15 @@ Section state_interpretation.
       assert (is_Some ((state_sockets σ) !! k)) as [z HSomez].
       { apply elem_of_dom. rewrite Hskt. apply elem_of_dom. by exists x. }
       iExists _, _.
-      iSplit; [done|]. 
       iSplit; [done|].
-      apply Hheaps in HSomey as ->.
-      apply Hskts in HSomez as ->.
-      rewrite fmap_empty.
+      iSplit; [done|].
+      apply lookup_total_correct in HSomey.
+      apply lookup_total_correct in HSomez.
+      simplify_eq.
       iFrame. }
     iSplitL "HipsCtx HPiu_auth".
     (* free_ips_coh *)
-    { by iApply (free_ips_coh_init with "[$]"). }
+    { by iApply (free_ips_coh_init_strong with "[$]"). }
     (* messages_resource_coh *)
     iApply messages_resource_coh_init.
     iFrame "#".
@@ -332,7 +232,9 @@ Section state_interpretation.
       rewrite fmap_empty. iFrame; iFrame "#"; eauto. }
     iSplitL "HipsCtx HPiu".
     (* free_ips_coh *)
-    { by iApply (free_ips_coh_init with "[$]"). }
+    { iApply (free_ips_coh_init with "[$]").
+      rewrite /ip_is_free. intros. assert (ip ≠ ip0) by set_solver.
+      rewrite Hste Hsce. rewrite !lookup_insert_ne; set_solver. }
     (* messages_resource_coh *)
     iApply messages_resource_coh_init.
     iFrame "#".
